

Wedge Product Expansion (3 vectors)

$$\begin{aligned} a \wedge b \wedge c = & \left(a_1 e_1 + a_2 e_2 + a_3 e_3 \right) \\ & \wedge \left(b_1 e_1 + b_2 e_2 + b_3 e_3 \right) \\ & \wedge \left(c_1 e_1 + c_2 e_2 + c_3 e_3 \right) \end{aligned}$$

$$\Delta = \begin{vmatrix} a_1 & a_2 & a_3 \\ b_1 & b_2 & b_3 \\ c_1 & c_2 & c_3 \end{vmatrix}$$

Wedge Product Expansion (3 vectors)

$$\begin{aligned} a \wedge b \wedge c = & (a_1 e_1 + a_2 e_2 + a_3 e_3) \\ & \wedge (b_1 e_1 + b_2 e_2 + b_3 e_3) \\ & \wedge (c_1 e_1 + c_2 e_2 + c_3 e_3) \end{aligned}$$

$$\Delta = \begin{vmatrix} a_1 & a_2 & a_3 \\ b_1 & b_2 & b_3 \\ c_1 & c_2 & c_3 \end{vmatrix}$$

Wedge Product Expansion (3 vectors)

$$\begin{aligned} a \wedge b \wedge c &= (a_1 e_1 + a_2 e_2 + a_3 e_3) \\ &\quad \wedge (b_1 e_1 + b_2 e_2 + b_3 e_3) \\ &\quad \wedge (c_1 e_1 + c_2 e_2 + c_3 e_3) \end{aligned}$$

$$\Delta = \begin{vmatrix} a_1 & a_2 & a_3 \\ b_1 & b_2 & b_3 \\ c_1 & c_2 & c_3 \end{vmatrix}$$

$$a \wedge b \wedge c = a_1(b_2 c_3 - b_3 c_2) e_1 \wedge e_{23}$$

Wedge Product Expansion (3 vectors)

$$\begin{aligned} a \wedge b \wedge c &= (a_1 e_1 + a_2 e_2 + a_3 e_3) \\ &\quad \wedge (b_1 e_1 + b_2 e_2 + b_3 e_3) \\ &\quad \wedge (c_1 e_1 + c_2 e_2 + c_3 e_3) \end{aligned}$$

$$\Delta = \begin{vmatrix} a_1 & a_2 & a_3 \\ b_1 & b_2 & b_3 \\ c_1 & c_2 & c_3 \end{vmatrix}$$

$$a \wedge b \wedge c = a_1(b_2 c_3 - b_3 c_2) e_1 \wedge e_{23}$$

$$\Delta = a_1(b_2 c_3 - b_3 c_2)$$

Wedge Product Expansion (3 vectors)

$$\begin{aligned} a \wedge b \wedge c &= (a_1 e_1 + a_2 e_2 + a_3 e_3) \\ &\quad \wedge (b_1 e_1 + b_2 e_2 + b_3 e_3) \\ &\quad \wedge (c_1 e_1 + c_2 e_2 + c_3 e_3) \end{aligned}$$

$$\Delta = \begin{vmatrix} a_1 & a_2 & a_3 \\ b_1 & b_2 & b_3 \\ c_1 & c_2 & c_3 \end{vmatrix}$$

$$a \wedge b \wedge c = a_1(b_2 c_3 - b_3 c_2) e_1 \wedge e_{23}$$

$$\Delta = a_1(b_2 c_3 - b_3 c_2)$$

Wedge Product Expansion (3 vectors)

$$\begin{aligned} a \wedge b \wedge c &= (a_1 e_1 + a_2 e_2 + a_3 e_3) \\ &\wedge (b_1 e_1 + b_2 e_2 + b_3 e_3) \\ &\wedge (c_1 e_1 + c_2 e_2 + c_3 e_3) \end{aligned}$$

$$\Delta = \begin{vmatrix} a_1 & a_2 & a_3 \\ b_1 & b_2 & b_3 \\ c_1 & c_2 & c_3 \end{vmatrix}$$

$$\begin{aligned} a \wedge b \wedge c &= a_1(b_2 c_3 - b_3 c_2) e_1 \wedge e_{23} \\ &+ a_2(b_1 c_3 - b_3 c_1) e_2 \wedge e_{13} \\ &+ a_3(b_1 c_2 - b_2 c_1) e_3 \wedge e_{12} \end{aligned}$$

$$\Delta = a_1(b_2 c_3 - b_3 c_2)$$

Wedge Product Expansion (3 vectors)

$$\begin{aligned} a \wedge b \wedge c &= (a_1 e_1 + a_2 e_2 + a_3 e_3) \\ &\wedge (b_1 e_1 + b_2 e_2 + b_3 e_3) \\ &\wedge (c_1 e_1 + c_2 e_2 + c_3 e_3) \end{aligned}$$

$$\Delta = \begin{vmatrix} a_1 & a_2 & a_3 \\ b_1 & b_2 & b_3 \\ c_1 & c_2 & c_3 \end{vmatrix}$$

$$\begin{aligned} a \wedge b \wedge c &= a_1(b_2 c_3 - b_3 c_2) e_1 \wedge e_{23} \\ &+ a_2(b_1 c_3 - b_3 c_1) e_2 \wedge e_{13} \\ &+ a_3(b_1 c_2 - b_2 c_1) e_3 \wedge e_{12} \end{aligned}$$

$$\begin{aligned} \Delta &= a_1(b_2 c_3 - b_3 c_2) \\ &- a_2(b_1 c_3 - b_3 c_1) \\ &+ a_3(b_1 c_2 - b_2 c_1) \end{aligned}$$

Wedge Product Expansion (3 vectors)

$$\begin{aligned} a \wedge b \wedge c &= (a_1 e_1 + a_2 e_2 + a_3 e_3) \\ &\wedge (b_1 e_1 + b_2 e_2 + b_3 e_3) \\ &\wedge (c_1 e_1 + c_2 e_2 + c_3 e_3) \end{aligned}$$

$$\Delta = \begin{vmatrix} a_1 & a_2 & a_3 \\ b_1 & b_2 & b_3 \\ c_1 & c_2 & c_3 \end{vmatrix}$$

$$\begin{aligned} a \wedge b \wedge c &= a_1(b_2 c_3 - b_3 c_2) e_1 \wedge e_{23} \\ &\quad + a_2(b_1 c_3 - b_3 c_1) e_2 \wedge e_{13} \end{aligned}$$

$$\begin{aligned} \Delta &= a_1(b_2 c_3 - b_3 c_2) \\ &\quad - a_2(b_1 c_3 - b_3 c_1) \end{aligned}$$

Wedge Product Expansion (3 vectors)

$$\begin{aligned} a \wedge b \wedge c &= (a_1 e_1 + a_2 e_2 + a_3 e_3) \\ &\wedge (b_1 e_1 + b_2 e_2 + b_3 e_3) \\ &\wedge (c_1 e_1 + c_2 e_2 + c_3 e_3) \end{aligned}$$

$$\Delta = \begin{vmatrix} a_1 & a_2 & a_3 \\ b_1 & b_2 & b_3 \\ c_1 & c_2 & c_3 \end{vmatrix}$$

$$\begin{aligned} a \wedge b \wedge c &= a_1(b_2 c_3 - b_3 c_2) e_1 \wedge e_{23} \\ &+ a_2(b_1 c_3 - b_3 c_1) e_2 \wedge e_{13} \\ &+ a_3(b_1 c_2 - b_2 c_1) e_3 \wedge e_{12} \end{aligned}$$

$$\begin{aligned} \Delta &= a_1(b_2 c_3 - b_3 c_2) \\ &\quad - a_2(b_1 c_3 - b_3 c_1) \end{aligned}$$

Wedge Product Expansion (3 vectors)

$$\begin{aligned} a \wedge b \wedge c &= (a_1 e_1 + a_2 e_2 + a_3 e_3) \\ &\wedge (b_1 e_1 + b_2 e_2 + b_3 e_3) \\ &\wedge (c_1 e_1 + c_2 e_2 + c_3 e_3) \end{aligned}$$

$$\Delta = \begin{vmatrix} a_1 & a_2 & a_3 \\ b_1 & b_2 & b_3 \\ c_1 & c_2 & c_3 \end{vmatrix}$$

$$\begin{aligned} a \wedge b \wedge c &= a_1(b_2 c_3 - b_3 c_2) e_1 \wedge e_{23} \\ &+ a_2(b_1 c_3 - b_3 c_1) e_2 \wedge e_{13} \\ &+ a_3(b_1 c_2 - b_2 c_1) e_3 \wedge e_{12} \end{aligned}$$

$$\begin{aligned} \Delta &= a_1(b_2 c_3 - b_3 c_2) \\ &- a_2(b_1 c_3 - b_3 c_1) \\ &+ a_3(b_1 c_2 - b_2 c_1) \end{aligned}$$

Wedge Product Expansion (3 vectors)

$$\begin{aligned} a \wedge b \wedge c &= (a_1 e_1 + a_2 e_2 + a_3 e_3) \\ &\quad \wedge (b_1 e_1 + b_2 e_2 + b_3 e_3) \\ &\quad \wedge (c_1 e_1 + c_2 e_2 + c_3 e_3) \end{aligned}$$

$$\Delta = \begin{vmatrix} a_1 & a_2 & a_3 \\ b_1 & b_2 & b_3 \\ c_1 & c_2 & c_3 \end{vmatrix}$$

$$\begin{aligned} a \wedge b \wedge c &= a_1(b_2 c_3 - b_3 c_2) e_1 \wedge e_{23} \\ &\quad + a_2(b_1 c_3 - b_3 c_1) e_2 \wedge e_{13} \\ &\quad + a_3(b_1 c_2 - b_2 c_1) e_3 \wedge e_{12} \\ &= \Delta e_{123} \end{aligned}$$

$$\begin{aligned} \Delta &= a_1(b_2 c_3 - b_3 c_2) \\ &\quad - a_2(b_1 c_3 - b_3 c_1) \\ &\quad + a_3(b_1 c_2 - b_2 c_1) \end{aligned}$$

Wedge Product Expansion (3 vectors)

$$\begin{aligned} a \wedge b \wedge c &= (a_1 e_1 + a_2 e_2 + a_3 e_3) \\ &\wedge (b_1 e_1 + b_2 e_2 + b_3 e_3) \\ &\wedge (c_1 e_1 + c_2 e_2 + c_3 e_3) \end{aligned}$$

$$\Delta = \begin{vmatrix} a_1 & a_2 & a_3 \\ b_1 & b_2 & b_3 \\ c_1 & c_2 & c_3 \end{vmatrix}$$

$$\begin{aligned} a \wedge b \wedge c &= a_1(b_2 c_3 - b_3 c_2) e_1 \wedge e_{23} \\ &+ a_2(b_1 c_3 - b_3 c_1) e_2 \wedge e_{13} \\ &+ a_3(b_1 c_2 - b_2 c_1) e_3 \wedge e_{12} \\ &= \Delta e_{123} \end{aligned}$$

$$\begin{aligned} \Delta &= a_1(b_2 c_3 - b_3 c_2) \\ &- a_2(b_1 c_3 - b_3 c_1) \\ &+ a_3(b_1 c_2 - b_2 c_1) \end{aligned}$$

Summary

$$\begin{vmatrix} a_1 & a_2 & a_3 \\ b_1 & b_2 & b_3 \\ c_1 & c_2 & c_3 \end{vmatrix} = +a_1 \begin{vmatrix} b_2 & b_3 \\ c_2 & c_3 \end{vmatrix} - a_2 \begin{vmatrix} b_1 & b_3 \\ c_1 & c_3 \end{vmatrix} + a_3 \begin{vmatrix} b_1 & b_2 \\ c_1 & c_2 \end{vmatrix}$$